Maintain application state in Broadcast

src/Broadcast.thy
@@ -17,7 +17,7 @@ record ('nodeid, 'op) message =
   msg_deps :: "'nodeid \<Rightarrow> nat"
   msg_op   :: "'op"
 
-type_synonym ('nodeid, 'op) node_state = "(('nodeid, 'op) message event, unit) node"
+type_synonym ('nodeid, 'op, 'state) node_state = "(('nodeid, 'op) message event, 'state option) node"
 
 definition filter_bcast :: "('nodeid, 'op) message event list \<Rightarrow> ('nodeid, 'op) message list" where
   "filter_bcast evts \<equiv> List.map_filter (\<lambda>e. case e of Broadcast m \<Rightarrow> Some m | _ \<Rightarrow> None) evts"
@@ -25,7 +25,7 @@ definition filter_bcast :: "('nodeid, 'op) message event list \<Rightarrow> ('no
 definition filter_deliv :: "('nodeid, 'op) message event list \<Rightarrow> ('nodeid, 'op) message list" where
   "filter_deliv evts \<equiv> List.map_filter (\<lambda>e. case e of Deliver m \<Rightarrow> Some m | _ \<Rightarrow> None) evts"
 
-definition causal_deps :: "('nodeid, 'op) node_state \<Rightarrow> 'nodeid \<Rightarrow> nat" where
+definition causal_deps :: "('nodeid, 'op, 'state) node_state \<Rightarrow> 'nodeid \<Rightarrow> nat" where
   "causal_deps state \<equiv> foldl
     (\<lambda>map msg. case msg_id msg of (node, seq) \<Rightarrow> map(node := seq))
     (\<lambda>n. 0) (filter_deliv (fst state))"
@@ -33,49 +33,61 @@ definition causal_deps :: "('nodeid, 'op) node_state \<Rightarrow> 'nodeid \<Rig
 definition deps_leq :: "('nodeid \<Rightarrow> nat) \<Rightarrow> ('nodeid \<Rightarrow> nat) \<Rightarrow> bool" where
   "deps_leq left right \<equiv> \<forall>node::'nodeid. left node \<le> right node"
 
-definition causally_ready :: "('nodeid, 'op) node_state \<Rightarrow> ('nodeid, 'op) message \<Rightarrow> bool" where
+definition causally_ready :: "('nodeid, 'op, 'state) node_state \<Rightarrow> ('nodeid, 'op) message \<Rightarrow> bool" where
   "causally_ready state msg \<equiv>
      deps_leq (msg_deps msg) (causal_deps state) \<and>
      (case msg_id msg of (sender, seq) \<Rightarrow> seq = Suc(causal_deps state sender))"
 
-definition next_msgid :: "'nodeid \<Rightarrow> ('nodeid, 'op) node_state \<Rightarrow> 'nodeid msgid" where
+definition next_msgid :: "'nodeid \<Rightarrow> ('nodeid, 'op, 'state) node_state \<Rightarrow> 'nodeid msgid" where
   "next_msgid sender state \<equiv> (sender, Suc (length (filter_bcast (fst state))))"
 
-definition valid_msgs :: "(('nodeid, 'op) node_state \<Rightarrow> 'op set) \<Rightarrow> 'nodeid \<Rightarrow> ('nodeid, 'op) node_state \<Rightarrow> ('nodeid, 'op) message set" where
-  "valid_msgs valid_ops sender state \<equiv>
+locale cbcast_protocol_base = executions _ valid_msg
+  for valid_msg :: "'nodeid \<Rightarrow> ('nodeid, 'op, 'state) node_state \<Rightarrow> ('nodeid, 'op) message set" +
+  fixes initial_state :: "'state"
+  and interp :: "'op \<Rightarrow> 'state \<rightharpoonup> 'state"
+  and valid_ops :: "'nodeid \<Rightarrow> 'state \<Rightarrow> 'op set"
+
+definition (in cbcast_protocol_base) valid_msgs ::
+  "'nodeid \<Rightarrow> ('nodeid, 'op, 'state) node_state \<Rightarrow> ('nodeid, 'op) message set" where
+  "valid_msgs sender state \<equiv> case snd state of None \<Rightarrow> {} | Some s \<Rightarrow>
      (\<lambda>oper. \<lparr>msg_id   = next_msgid sender state,
               msg_deps = causal_deps state,
               msg_op   = oper\<rparr>
-     ) ` valid_ops state"
+     ) ` valid_ops sender s"
 
-definition protocol_send ::
-  "'nodeid \<Rightarrow> ('nodeid, 'op) node_state \<Rightarrow> ('nodeid, 'op) message \<Rightarrow> ('nodeid, 'op) node_state" where
-  "protocol_send sender state msg \<equiv> ([Broadcast msg, Deliver msg], ())"
+definition (in cbcast_protocol_base) protocol_send ::
+  "'nodeid \<Rightarrow> ('nodeid, 'op, 'state) node_state \<Rightarrow> ('nodeid, 'op) message \<Rightarrow> ('nodeid, 'op, 'state) node_state" where
+  "protocol_send sender state msg \<equiv> case snd state of None \<Rightarrow> ([], None) | Some s \<Rightarrow>
+     ([Broadcast msg, Deliver msg], interp (msg_op msg) s)"
 
-definition protocol_recv ::
-  "'nodeid \<Rightarrow> ('nodeid, 'op) node_state \<Rightarrow> ('nodeid, 'op) message \<Rightarrow> ('nodeid, 'op) node_state" where
+definition (in cbcast_protocol_base) protocol_recv ::
+  "'nodeid \<Rightarrow> ('nodeid, 'op, 'state) node_state \<Rightarrow> ('nodeid, 'op) message \<Rightarrow> ('nodeid, 'op, 'state) node_state" where
   "protocol_recv recipient state msg \<equiv>
-     if causally_ready state msg then ([Deliver msg], ()) else ([], ())"
+     if causally_ready state msg
+     then case snd state of
+       None   \<Rightarrow> ([], None) |
+       Some s \<Rightarrow> ([Deliver msg], interp (msg_op msg) s)
+     else ([], snd state)"
 
-locale cbcast_protocol_base = executions "\<lambda>n. ()" valid_msg protocol_send protocol_recv
-  for valid_msg :: "nat \<Rightarrow> (nat, 'op) message event list \<times> unit \<Rightarrow> (nat, 'op) message set" +
-  fixes valid_ops :: "(nat, 'op) node_state \<Rightarrow> 'op set"
-
-locale cbcast_protocol = cbcast_protocol_base "valid_msgs valid_ops" valid_ops
-  for valid_ops :: "(nat, 'op) message event list \<times> unit \<Rightarrow> 'op set" +
-  fixes config :: "(nat, (nat, 'op) message, (nat, 'op) message event, unit) system"
+locale cbcast_protocol = cbcast_protocol_base
+  "\<lambda>n. Some initial_state"
+  "cbcast_protocol_base.protocol_send interp"
+  "cbcast_protocol_base.protocol_recv interp"
+  "cbcast_protocol_base.valid_msgs valid_ops" _ _ valid_ops
+  for valid_ops :: "'nodeid \<Rightarrow> 'state \<Rightarrow> 'op set" +
+  fixes config :: "('nodeid, ('nodeid, 'op) message, ('nodeid, 'op) message event, 'state option) system"
   assumes valid_execution: "execution config"
 
-definition (in cbcast_protocol) history :: "nat \<Rightarrow> (nat, 'op) message event list" where
+definition (in cbcast_protocol) history :: "'nodeid \<Rightarrow> ('nodeid, 'op) message event list" where
   "history i \<equiv> fst (snd config i)"
 
-definition (in cbcast_protocol) all_messages :: "(nat, 'op) message set" where
+definition (in cbcast_protocol) all_messages :: "('nodeid, 'op) message set" where
   "all_messages \<equiv> fst config"
 
-definition (in cbcast_protocol) broadcasts :: "nat \<Rightarrow> (nat, 'op) message list" where
+definition (in cbcast_protocol) broadcasts :: "'nodeid \<Rightarrow> ('nodeid, 'op) message list" where
   "broadcasts i \<equiv> List.map_filter (\<lambda>e. case e of Broadcast m \<Rightarrow> Some m | _ \<Rightarrow> None) (history i)"
 
-definition (in cbcast_protocol) deliveries :: "nat \<Rightarrow> (nat, 'op) message list" where
+definition (in cbcast_protocol) deliveries :: "'nodeid \<Rightarrow> ('nodeid, 'op) message list" where
   "deliveries i \<equiv> List.map_filter (\<lambda>e. case e of Deliver m \<Rightarrow> Some m | _ \<Rightarrow> None) (history i)"
 
 
@@ -84,14 +96,15 @@ subsection\<open>Proof that this protocol satisfies the causal network assumptio
 lemma (in cbcast_protocol) broadcast_origin:
   assumes "history i = xs @ Broadcast msg # ys"
     and "Broadcast msg \<notin> set xs"
-  shows "\<exists>pre before after suf oper evts.
+  shows "\<exists>pre before after suf state oper evts.
     config_evolution config (pre @ [before, after] @ suf) \<and>
-    oper \<in> valid_ops (snd before i) \<and>
+    snd (snd before i) = Some state \<and>
+    oper \<in> valid_ops i state \<and>
     msg = \<lparr>msg_id   = next_msgid i (snd before i),
            msg_deps = causal_deps (snd before i),
            msg_op   = oper\<rparr> \<and>
     evts = fst (snd before i) @ [Broadcast msg, Deliver msg] \<and>
-    after = (insert msg (fst before), (snd before)(i := (evts, ()))) \<and>
+    after = (insert msg (fst before), (snd before)(i := (evts, interp (msg_op msg) state))) \<and>
     fst (snd before i) = xs"
   using assms valid_execution apply -
   apply(frule config_evolution_exists, erule exE)
@@ -106,29 +119,33 @@ lemma (in cbcast_protocol) broadcast_origin:
   apply(simp add: case_prod_beta protocol_send_def split: if_split_asm)
   apply(erule unpack_let)
   apply(subgoal_tac "sender=i") prefer 2 apply force
+  apply(case_tac "snd (snd before i) = None", force)
   apply(subgoal_tac "fst (snd after i) = fst (snd before i) @ [Broadcast msga, Deliver msga]")
   prefer 2 apply force
   apply(subgoal_tac "msga=msg") prefer 2 apply simp
-  apply(subgoal_tac "msg \<in> valid_msgs valid_ops i (snd before i)")
+  apply(subgoal_tac "msg \<in> valid_msgs i (snd before i)")
   prefer 2 apply(simp add: some_set_memb)
   apply(rule_tac x="fst before" in exI, rule_tac x="snd before" in exI)
   apply(rule_tac x="fst after" in exI, rule_tac x="snd after" in exI)
   apply(rule conjI, force)
+  apply(rule_tac x="the (snd (snd before i))" in exI)
+  apply(rule conjI, force)
   apply(rule_tac x="msg_op msg" in exI)
-  apply(subgoal_tac "valid_ops (snd before i) \<noteq> {}")
-  prefer 2 apply(simp add: valid_msgs_def)
+  apply(subgoal_tac "valid_ops i (the (snd (snd before i))) \<noteq> {}")
+  prefer 2 apply(simp add: valid_msgs_def, force)
   apply(subgoal_tac "msg \<in> (\<lambda>oper.
              \<lparr>msg_id   = next_msgid i (snd before i),
               msg_deps = causal_deps (snd before i),
-              msg_op   = oper\<rparr>) ` valid_ops (snd before i)")
-  prefer 2 apply (simp add: valid_msgs_def)
-  apply(subgoal_tac "msg_op msg \<in> valid_ops (snd before i)")
+              msg_op   = oper\<rparr>) ` valid_ops i (the (snd (snd before i)))")
+  prefer 2 apply(simp add: valid_msgs_def, force)
+  apply(subgoal_tac "msg_op msg \<in> valid_ops i (the (snd (snd before i)))")
   prefer 2 apply force
   apply((rule conjI, force)+, force)
   apply(simp add: recv_step_def protocol_recv_def case_prod_beta split: if_split_asm)
-  apply(erule unpack_let)+
+    apply(erule unpack_let)+
   apply(subgoal_tac "recipient=i")
-  apply force+
+  apply(case_tac "causally_ready (snd before recipient) msga")
+  apply(case_tac "snd (snd before i) = None", force+)
 done
 
 lemma (in cbcast_protocol) broadcast_msg_eq:
@@ -146,10 +163,14 @@ lemma (in cbcast_protocol) broadcast_msg_eq:
   apply(insert valid_execution, drule config_evolution_exists, erule exE)
   apply(drule message_origin, simp, (erule exE)+, (erule conjE)+)
   apply(rule_tac x=sender in exI)
+  apply(case_tac "snd (snd before sender) = None", simp add: valid_msgs_def)
+  apply(subgoal_tac "Broadcast msg \<in> set evts") defer
+  apply(simp add: protocol_send_def, force)
   apply(subgoal_tac "Broadcast msg \<in> set (fst (snd config sender))")
   apply(simp add: history_def)
   apply(subgoal_tac "\<exists>xs. fst (snd after sender) @ xs = fst (snd config sender)")
-  apply(simp add: protocol_send_def, metis in_set_conv_decomp)
+  apply(simp add: protocol_send_def)
+  apply(metis (no_types, lifting) append.assoc append_Cons in_set_conv_decomp)
   apply(insert history_monotonic)[1]
   apply(erule_tac x="config" in meta_allE)
   apply(erule_tac x="pre @ [before]" in meta_allE)
@@ -262,12 +283,23 @@ lemma (in cbcast_protocol) msg_id_unique:
   using broadcast_node_id apply fastforce+
 done
 
-context cbcast_protocol begin
-sublocale causal: causal_network history msg_id
-  apply standard
-  prefer 4 apply(simp add: msg_id_unique)
-  oops
+locale cbcast_with_ops = cbcast_protocol _ _ valid_ops
+  for valid_ops :: "nat \<Rightarrow> 'state \<Rightarrow> 'op set"
+begin
 
+  definition op_history :: "nat \<Rightarrow> (nat msgid \<times> 'op) event list" where
+    "op_history i \<equiv> map (\<lambda>evt. case evt of
+        Broadcast msg \<Rightarrow> Broadcast (msg_id msg, msg_op msg) |
+        Deliver   msg \<Rightarrow> Deliver   (msg_id msg, msg_op msg)
+      ) (history i)"
+    
+  definition valid_op_msgs :: "nat \<Rightarrow> 'state \<Rightarrow> (nat msgid \<times> 'op) set" where
+    "valid_op_msgs node state \<equiv> undefined"
+
+  sublocale axiomatic: network_with_constrained_ops op_history interp initial_state valid_op_msgs
+  apply standard
+  prefer 4 apply(simp add: op_history_def msg_id_unique)
+  oops
 end
 
 end
